---
tags:
  - Mathe
---
*Marvin Baeumer* **2023-11-15 09:26**

---
$$(a \cdot b) \mod m = (a \mod m \cdot b \mod m) \mod m$$
$$(a^b) \mod m = (a \mod m)^b \mod m$$
### Beispiele 
$$
\begin{matrix}
a & 8^9 \mod 7 & = & 1^9 \mod 7
\end{matrix}
$$
$$
\begin{matrix}
b & 6^9 \mod 7 & = & - 1^9\mod 7 \\
& & = & 6 & \\
\end{matrix}
$$
$$
\begin{matrix}
c & 54^{16} \mod 55 & = & - 1^{16}\mod 7 \\
& & = & 54 & \\
\end{matrix}
$$
$$
\begin{matrix}
d & 3^{333} \mod 26 & = & 3^{3 \cdot 111} \mod 26 \\
& & = & (27 \cdot 27 \cdot 27) \mod 26 & \\
& & = & 27 \mod 26 & \\
& & = & 1 &
\end{matrix}
$$
$$
\begin{matrix}
e & 2^{268} \mod 17 & = & 3^3 \cdot 3^3 \cdot 3^3 \mod 26 \\
& & = & (27 \cdot 27 \cdot 27) \mod 26 & \\
& & = & 27 \mod 26 & \\
& & = & 1 &
\end{matrix}
$$